Renovate StaticFun a bit.
The functor is gone, and instead StaticFun exports two more general
operators, one for defining a partial map by a tree, and one for
extracting the theorems from an existing partial map definition.

The extraction process uses simplification in a more conservative
manner than before, and is guaranteed to produce exactly the
expected theorems.

tools/c-parser/StaticFun.thy
@@ -10,11 +10,7 @@
 
 theory StaticFun
 imports
-  "../../lib/StringOrd"
-  "../../lib/WordLib"
-  "~~/src/HOL/Library/Numeral_Type"
-keywords
-  "test_tree" "test_tree2" :: thy_decl
+  Main
 begin
 
 datatype ('a, 'b) Tree = Node 'a 'b "('a, 'b) Tree" "('a, 'b) Tree" | Leaf
@@ -27,74 +23,134 @@ where
                                       else if fn x < fn y then lookup_tree l fn x
                                       else lookup_tree r fn x)"
 
-definition
-  tree_gives_vals :: "('a, 'b) Tree \<Rightarrow> ('a \<Rightarrow> 'c :: linorder) \<Rightarrow> ('a \<rightharpoonup> 'b) \<Rightarrow> 'c set \<Rightarrow> bool"
+definition optional_strict_range :: "('a :: linorder) option \<Rightarrow> 'a option \<Rightarrow> 'a set"
 where
- "tree_gives_vals T ord f S \<equiv> \<forall>x. (ord x \<in> S) \<longrightarrow> f x = lookup_tree T ord x"
+  "optional_strict_range x y = {z. (x = None \<or> the x < z) \<and> (y = None \<or> z < the y)}"
 
-lemma tree_gives_valsI:
- "\<lbrakk> f \<equiv> lookup_tree T ord \<rbrakk> \<Longrightarrow> tree_gives_vals T ord f UNIV"
-  by (simp add: tree_gives_vals_def)
+lemma optional_strict_range_split:
+  "z \<in> optional_strict_range x y
+    \<Longrightarrow> optional_strict_range x (Some z) = ({..< z} \<inter> optional_strict_range x y)
+        \<and> optional_strict_range (Some z) y = ({z <..} \<inter> optional_strict_range x y)"
+  by (auto simp add: optional_strict_range_def)
 
-lemma tree_gives_valsD:
-  assumes "tree_gives_vals (Node y v l r) ord f S"
-  shows "ord y \<in> S \<longrightarrow> f y = Some v"
-  and   "tree_gives_vals l ord f (S \<inter> {..<ord y})"
-  and   "tree_gives_vals r ord f (S \<inter> {ord y<..})"
-  using assms
-  apply -
-    apply (simp add: tree_gives_vals_def)+
+lemma optional_strict_rangeI:
+  "z \<in> optional_strict_range None None"
+  "z < y \<Longrightarrow> z \<in> optional_strict_range None (Some y)"
+  "x < z \<Longrightarrow> z \<in> optional_strict_range (Some x) None"
+  "x < z \<Longrightarrow> z < y \<Longrightarrow> z \<in> optional_strict_range (Some x) (Some y)"
+  by (simp_all add: optional_strict_range_def)
+
+definition
+  tree_eq_fun_in_range :: "('a, 'b) Tree \<Rightarrow> ('a \<Rightarrow> 'c :: linorder) \<Rightarrow> ('a \<rightharpoonup> 'b) \<Rightarrow> 'c set \<Rightarrow> bool"
+where
+ "tree_eq_fun_in_range T ord f S \<equiv> \<forall>x. (ord x \<in> S) \<longrightarrow> f x = lookup_tree T ord x"
+
+lemma tree_eq_fun_in_range_from_def:
+  "\<lbrakk> f \<equiv> lookup_tree T ord \<rbrakk>
+    \<Longrightarrow> tree_eq_fun_in_range T ord f (optional_strict_range None None)"
+  by (simp add: tree_eq_fun_in_range_def)
+
+lemma tree_eq_fun_in_range_split:
+  "tree_eq_fun_in_range (Node z v l r) ord f (optional_strict_range x y)
+    \<Longrightarrow> ord z \<in> optional_strict_range x y
+    \<Longrightarrow> tree_eq_fun_in_range l ord f (optional_strict_range x (Some (ord z)))
+        \<and> f z = Some v
+        \<and> tree_eq_fun_in_range r ord f (optional_strict_range (Some (ord z)) y)"
+  apply (simp add: tree_eq_fun_in_range_def optional_strict_range_split)
   apply fastforce
   done
 
-lemma tree_gives_vals_setonly_cong:
-  "\<lbrakk> S = S' \<rbrakk> \<Longrightarrow> tree_gives_vals T ord f S = tree_gives_vals T ord f S'"
-  by simp
+ML {*
 
-lemma tree_vals_set_Int_simps:
-  "UNIV \<inter> S = S"
-  "({..<(x :: 'a :: linorder)} \<inter> {..<y}) = (if x < y then {..<x} else {..<y})"
-  "({x<..} \<inter> {y<..}) = (if x < y then {y<..} else {x<..})"
-  "({..<x} \<inter> {y<..}) = ({y<..} \<inter> {..<x})"
-  "(({y<..} \<inter> {..<x}) \<inter> {z<..}) = ((if y < z then {z<..} else {y<..}) \<inter> {..<x})"
-  "(({y<..} \<inter> {..<x}) \<inter> {..<z}) = ((if x < z then {..<x} else {..<z}) \<inter> {y<..})"
-  by auto
+structure StaticFun = struct
 
-lemmas tree_vals_set_simps =
-  Int_iff greaterThan_iff lessThan_iff simp_thms UNIV_I
-  tree_vals_set_Int_simps if_True if_False
+(* Actually build the tree -- theta (n lg(n)) *)
+fun build_tree' _ mk_leaf [] = mk_leaf
+  | build_tree' mk_node mk_leaf xs = let
+    val len = length xs
+    val (ys, zs) = chop (len div 2) xs
+  in case zs of [] => error "build_tree': impossible"
+    | ((a, b) :: zs) => mk_node a b (build_tree' mk_node mk_leaf ys)
+        (build_tree' mk_node mk_leaf zs)
+  end
 
-lemma int_0_less_1: "0 < (1::int)" by simp
+fun build_tree ord xs = case xs of [] => error "build_tree : empty"
+  | (idx, v) :: _ => let
+    val idxT = fastype_of idx
+    val vT = fastype_of v
+    val treeT = Type (@{type_name StaticFun.Tree}, [idxT, vT])
+    val mk_leaf = Const (@{const_name StaticFun.Leaf}, treeT)
+    val node = Const (@{const_name StaticFun.Node},
+        idxT --> vT --> treeT --> treeT --> treeT)
+    fun mk_node a b l r = node $ a $ b $ l $ r
+    val lookup = Const (@{const_name StaticFun.lookup_tree},
+        treeT --> fastype_of ord --> idxT
+            --> Type (@{type_name option}, [vT]))
+  in
+    lookup $ (build_tree' mk_node mk_leaf xs) $ ord
+  end
 
-lemmas int_simpset = arith_simps rel_simps id_apply arith_special int_0_less_1
+fun define_partial_map_tree name mappings ord ctxt = let
+    val tree = build_tree ord mappings
+  in Local_Theory.define
+    ((name, NoSyn), ((Thm.def_binding name, []), tree)) ctxt
+    |> apfst (apsnd snd)
+  end
 
-ML_file "isa_termstypes.ML"
-ML_file "static-fun.ML"
+fun prove_partial_map_thms thm ctxt = let
+    val init = thm RS @{thm tree_eq_fun_in_range_from_def}
+    fun rec_tree thm = case concl_of thm of
+    @{term Trueprop} $ (Const (@{const_name tree_eq_fun_in_range}, _)
+        $ (Const (@{const_name Node}, _) $ z $ v $ _ $ _) $ _ $ _ $ _) => let
+        val t' = thm RS @{thm tree_eq_fun_in_range_split}
+        val solve_simp_tac = SUBGOAL (fn (t, i) =>
+            (simp_tac ctxt THEN_ALL_NEW SUBGOAL (fn (t', _) =>
+                raise TERM ("prove_partial_map_thms: unsolved", [t, t']))) i)
+        val r = t' |> (resolve_tac @{thms optional_strict_rangeI}
+            THEN_ALL_NEW solve_simp_tac) 1 |> Seq.hd
+        val l = r RS @{thm conjunct1}
+        val kr = r RS @{thm conjunct2}
+        val k = kr RS @{thm conjunct1}
+        val r = kr RS @{thm conjunct2}
+      in rec_tree l @ [((z, v), k)] @ rec_tree r end
+    | _ => []
+  in rec_tree init end
 
-(*
-test_tree "gamma" 100
-locale foo =
-  fixes x :: int
-;
-context foo
-begin
-;
- test_tree "gamma" 100
+fun define_tree_and_save_thms name names mappings ord exsimps ctxt = let
+    val ((tree, def_thm), ctxt) = define_partial_map_tree name mappings ord ctxt
+    val thms = prove_partial_map_thms def_thm (ctxt addsimps exsimps)
+    val (idents, thms) = map_split I thms
+    val _ = map (fn ((x, y), (x', y')) => (x aconv x' andalso y aconv y')
+        orelse raise TERM ("define_tree_and_thms: different", [x, y, x', y']))
+        (mappings ~~ idents)
+    val (_, ctxt) = Local_Theory.notes
+        (map (fn (s, t) => ((Binding.name s, []), [([t], [])]))
+        (names ~~ thms)) ctxt
+  in (tree, ctxt) end
 
-Timing:
+fun define_tree_and_thms_with_defs name names key_defs opt_values ord ctxt = let
+    val data = names ~~ (key_defs ~~ opt_values)
+        |> map_filter (fn (_, (_, NONE)) => NONE | (nm, (thm, SOME v))
+            => SOME (nm, (fst (Logic.dest_equals (concl_of thm)), v)))
+    val (names, mappings) = map_split I data
+  in define_tree_and_save_thms name names mappings ord key_defs ctxt end
 
-  test_tree "gamma" 10000
+end
 
-  int/\<longrightarrow>/700 = 32.582
-  nat/\<longrightarrow>/700 = 49.643
-  int/700    = 33. \<dots>
-  int/simps/700 = 6.123
-  int/simps/5000 = 65.184 secs
-  int/simps/10000 = 154.166
-  int/allsimps/700 = 3.00
-  int/allsimps/5000 = 26.00 (TS: simps ran in 50sec on mine)
-  string/allsimps/700 = 5.76
-  string/allsimps/5000 = 47.53
- *)
+*}
+
+(* testing
+
+local_setup {* StaticFun.define_tree_and_save_thms @{binding tree}
+  ["one", "two", "three"]
+  [(@{term "Suc 0"}, @{term "Suc 0"}),
+    (@{term "2 :: nat"}, @{term "15 :: nat"}),
+    (@{term "3 :: nat"}, @{term "1 :: nat"})]
+  @{term "id :: nat \<Rightarrow> nat"}
+  #> snd
+*}
+print_theorems
+
+*)
 
 end
